notes

coq/denot/definitions.v
@@ -48,11 +48,14 @@ Open Scope monad_scope.
 Import SetNotations.
 Local Open Scope set_scope.
 
+(* Sets of Values:   P Value === Value -> Prop *)
+
 Inductive Value : Type :=
   (* natural number *)
   | v_nat : nat -> Value
 
   (* one entry in a function's table *)
+  (* list Value is Finite set of values here *)
   | v_map : list Value -> Value -> Value
 
   (* trivial function value, evaluated to a value but never applied *)
@@ -64,6 +67,15 @@ Inductive Value : Type :=
   (* dynamic type error *)
   | v_wrong : Value
 .
+
+(* 
+
+Denotation of Identity function (\x.x):
+
+ {  v_map (v_nat 1 :: nil) (v_nat 1), (2 :: nil) |-> 2, 3 |-> 3 
+ } 
+
+ *)
 
 #[export] Hint Constructors Value : core.
 
@@ -106,13 +118,135 @@ Definition NIL : P Value := ⌈ v_list nil ⌉.
 Definition CONS : P Value -> P Value -> P Value := 
   fun V W x => 
     match x with 
-    | v_list (v :: w) => (v ∈ V) /\ (v_list w ∈ W)
+    | v_list (v :: w) => (v ∈ V) /\ (v_list w ∈ W)  (* v should not be wrong *)
+(*     | v_wrong => v_wrong ∈ V *)
     | _ => False
     end.
 
 Definition Λ : (P Value -> P Value) -> P Value :=
   fun f => fun v => match v with 
           | (V ↦ w) => (w ∈ f (mem V)) /\ valid_mem V  (* CBV *)
+          | v_fun => True
+          | _ => False
+          end.
+
+(* ------------ APPLY ----------------- *)
+
+(* It is a little easier to specify this as an inductive relation 
+   than as a function. The cases don't overlap, but we don't need
+   to know that at definition time.
+*)
+
+
+(* When does APPLY diverge? (i.e. there is no w, s.t. APPLY D1 D2 w holds)
+    - D1 is empty
+    - D2 is empty
+    - D1 contains a vfun or V ↦ x, but cannot be applied to D2
+           << should this be empty or wrong??? >> 
+
+   When does APPLY propagate wrong?
+    - wrong in D1 or D2  (FUNWRONG / ARGWRONG) 
+    - V ↦ wrong in D1 and valid V in D2  (BETA case)
+
+   When does APPLY create a new wrong? 
+    - D1 contains a successful Value that is not a v_fun, v_map or v_list  (APPWRONG)
+    - D1 contains a v_list and D2 contains a successful Value that is not a nat (PROJWRONG)
+           
+*)
+
+Inductive applicable : Value -> Prop :=
+  | a_fun  : applicable v_fun
+  | a_list : forall VS, applicable (v_list VS)
+  | a_map  : forall V w, applicable (v_map V w).
+
+#[export] Hint Constructors applicable : core.
+
+Inductive APPLY : P Value -> P Value -> (Value -> Prop) :=
+  | FUNWRONG : forall D1 D2,
+     (v_wrong ∈ D1) ->
+     APPLY D1 D2 v_wrong
+  | ARGWRONG : forall D1 D2,
+     (v_wrong ∈ D2) ->
+     APPLY D1 D2 v_wrong
+  | BETA : forall D1 D2 w V,
+     (V ↦ w ∈ D1) -> (mem V ⊆ D2) -> valid_mem V ->
+     APPLY D1 D2 w
+  | PROJ   : forall D1 D2 w VS k, 
+     (v_list VS ∈ D1) -> (v_nat k ∈ D2) -> nth_error VS k = Some w ->
+     APPLY D1 D2 w
+  | APPWRONG : forall D1 D2 x, 
+      x ∈ D1 -> success x -> not (applicable x) ->      
+      APPLY D1 D2 v_wrong
+  | PROJWRONG : forall D1 D2 VS x, 
+     (v_list VS ∈ D1) -> 
+     (x ∈ D2) -> success x ->
+     (forall k, x <> (v_nat k)) ->
+     APPLY D1 D2 v_wrong. 
+
+(* Need to add out of bounds *)
+
+Infix "▩" := APPLY (at level 90).
+
+
+#[export] Hint Constructors APPLY : core.
+
+Definition ADD : P Value :=
+  fun w => 
+    match w with 
+    | (V ↦ v_nat k) => 
+        exists i j, ((v_list (v_nat i :: v_nat j :: nil)) ∈ mem V) /\ k = i + j
+    | V ↦ v_wrong => 
+        not (exists i j, v_list (v_nat i :: v_nat j :: nil) ∈ mem V) /\ valid_mem V
+    | _ => False
+    end.
+
+(* ------------------------------------------------------- *)
+
+Definition Rho := Env (P Value).
+
+Ltac gather_atoms ::=
+  let A := gather_atoms_with (fun x : vars => x) in
+  let B := gather_atoms_with (fun x : var => {{ x }}) in
+  let C := gather_atoms_with (fun x => fv_tm x) in
+  let D := gather_atoms_with (fun x : list (atom * P Value) => dom x) in
+  let E := gather_atoms_with (fun x : Rho => dom x) in
+  constr:(A \u B \u C \u D \u E).
+
+Module EnvNotations.
+Notation "ρ ⋅ x" := (Env.access ⌈ v_wrong ⌉ ρ x) (at level 50).
+Infix "⊔e" := (Env.map2 Union) (at level 60).
+Infix "⊆e" := (Env.Forall2 Included) (at level 50).
+End EnvNotations.
+Import EnvNotations.
+
+(* ------------------------------------------------------- *)
+
+Definition nonempty_env : Rho -> Type := Env.ForallT nonemptyT.
+
+Definition valid_env : Rho -> Type := Env.ForallT valid. 
+
+Definition sub_env : Rho -> Rho -> Prop := Env.Forall2 Included.
+
+Definition same_env : Rho -> Rho -> Prop := Env.Forall2 Same_set.
+
+(* ------------------------------------------------------- *)
+
+Import LCNotations.
+Open Scope tm.
+
+
+
+(* Denotation function *)
+(* `n` is is a termination metric. *)
+Fixpoint denot_n (n : nat) (a : tm) (ρ : Rho) : P Value :=
+  match n with
+  | O => fun _ => False
+  | S m => 
+     match a with 
+     | var_b _ => ⌈ v_wrong ⌉
+     | var_f x => ρ ⋅ x 
+     | app t u   => 
+         v1 <-  valid_mem V  (* CBV *)
           | v_fun => True
           | _ => False
           end.
@@ -219,9 +353,11 @@ Definition same_env : Rho -> Rho -> Prop := Env.Forall2 Same_set.
 Import LCNotations.
 Open Scope tm.
 
+
+
 (* Denotation function *)
 (* `n` is is a termination metric. *)
-Fixpoint denot_n (n : nat) (a : tm) (ρ : Rho) : P Value :=
+Fixpoint denot_n (n : nat) (a : tm) (ρ : Rho) : M (P Value) :=
   match n with
   | O => fun _ => False
   | S m => 
